git-svn-id: svn+ssh://scm.gforge.inria.fr/svn/coqcert/trunk/cic-model@110 7b0040dd-6dd6-45fd-888d-7922243e4794

CCTnat.v
@@ -1,8 +1,10 @@
 Require Import Models.
 Require Import GenModel.
 Require Import ModelZF.
+Require Import ZFnats.
 Require Import ZFcoc.
 Require Import ZF.
+Require Import ZFrepl.
 Import IZF.
 
 Module BuildModel := GenModel.MakeModel(CCM).
@@ -11,61 +13,513 @@ Import T.
 Import J.
 Import CCM.
 
-
+Definition T : term.
+left; exists (fun _ => N); do 2 red; reflexivity.
+Defined.
 
 Definition Zero : term.
-left; exists (fun _ => empty); do 2 red; reflexivity.
-Defined.
-
-Definition Succ : term.
-left; exists (fun _ => lam (singl empty) (fun x => x)); do 2 red; reflexivity.
-Defined.
-
-Definition NatRec (f g n:term) : term.
-left; exists (fun i => int f i);
-do 2 red; intros; rewrite H; reflexivity.
-Defined.
-
-Definition T : term.
-left; exists (fun _ => singl empty); do 2 red; reflexivity.
+left; exists (fun _ => zero); do 2 red; reflexivity.
 Defined.
 
 Lemma typ_0 : forall e, typ e Zero T.
-do 2 red; simpl; intros e i H; apply singl_intro.
+do 2 red; simpl; intros e i H; apply zero_typ.
 Qed.
 
-Lemma typ_S : forall e, typ e Succ (Prod T (lift 1 T)).
-do 2 red; simpl; intros e i H. apply prod_intro.
-  red. intros y1 y2 H0 H1; exact H1.
-  red; reflexivity.
-  intros x H0; exact H0.
+Definition Succ : term -> term.
+intro n; left; exists (fun i => succ (int n i)). 
+do 2 red; intros. rewrite H; reflexivity. 
+Defined.
+
+Lemma typ_S : forall e t, typ e t T -> typ e (Succ t) T.
+do 2 red; simpl; intros. apply succ_typ.
+apply H; apply H0.
 Qed.
+
+(*Definition Succ : term.
+left; exists (fun _ => lam N succ). 
+do 2 red; intros. reflexivity. 
+Defined.
+
+Lemma typ_S : forall e t, typ e t T ->
+  typ e Succ (Prod T (lift 1 T)).
+do 2 red; simpl; intros. apply prod_intro.
+ repeat red; intros. rewrite H2. reflexivity.
+ 
+ repeat red; reflexivity.
+
+ apply succ_typ.
+Qed.*)
+
+
+Definition NREC f g n y :=
+  forall P, 
+  Proper (eq_set ==> eq_set ==> iff) P ->
+  P zero f -> (forall m t, P m t -> P (succ m) (g m t)) -> P n y.
+
+Instance NREC_morph : 
+  Proper (eq_set ==> (eq_set ==> eq_set ==> eq_set) ==> eq_set ==> eq_set ==> iff) NREC.
+repeat red; split; intros.
+ unfold NREC; intros. 
+ rewrite <- H1; rewrite <- H2; apply H3; auto.
+  rewrite H; auto.
+
+  repeat red in H0. 
+  intros m t; rewrite (H0 _ _ (reflexivity m) _ _ (reflexivity t)).
+  apply H6.
+
+ unfold NREC; intros.
+ rewrite H1, H2. apply H3; auto.
+ rewrite <- H; auto.
+ 
+ repeat red in H0.
+ intros m t; rewrite <- (H0 _ _ (reflexivity m) _ _ (reflexivity t)).
+ apply H6.
+Qed.
+
+Lemma NREC_inv : forall f g n y,
+  n \in N ->
+  morph2 g ->
+  NREC f g n y ->
+  n \in N /\
+  NREC f g n y /\
+  (n == zero -> y == f) /\
+  (forall m, m \in N -> n == succ m -> exists2 z, NREC f g m z & y == g m z).
+intros. pattern n, y. apply H1. 
+ do 3 red; intros.
+ apply and_iff_morphism.
+  rewrite H2; reflexivity.
+  
+  apply and_iff_morphism.
+   rewrite H2; rewrite H3; reflexivity.
+
+   apply and_iff_morphism.
+    rewrite H3; rewrite H2; reflexivity.
+
+    apply fa_morph; intros. rewrite H2. 
+    apply fa_morph; intros. apply fa_morph; intros. 
+    apply ex2_morph; red.
+     reflexivity.
+   
+     intros. rewrite H3. reflexivity.
+
+ split; try split; try split; intros.
+  apply zero_typ.  
+
+  red; intro; auto.
+
+  reflexivity.
+
+  symmetry in H3; apply discr in H3; contradiction.
+
+ intros; split; try split; try split; intros; destruct H2.
+  apply succ_typ; auto.
+  
+  destruct H3. red; intros. apply H7. apply H3; auto.
+
+  apply discr in H3; contradiction.
+
+  apply succ_inj in H4; auto. exists t; rewrite <- H4.
+   destruct H5; assumption.
+
+   reflexivity.
+Qed.
+   
+  
+Lemma NREC_choice : forall f g n,
+  n \in N ->
+  morph2 g ->
+  uchoice_pred (NREC f g n).
+Proof.
+split;try split; intros.
+ unfold NREC; intros; rewrite <- H1; apply H2; auto.
+
+ elim H using N_ind; intros.
+  destruct H3. exists x.
+  unfold NREC; intros; rewrite <- H2; apply H3; auto.
+
+  exists f. unfold NREC; auto.
+  
+  destruct H2. exists (g n0 x). 
+  red; intros. apply H5. apply H2; auto.
+
+ revert x x' H1 H2. elim H using N_ind; intros.
+  apply H3.
+   red; intros; rewrite H2; apply H4; auto.
+   
+   red; intros; rewrite H2; apply H5; auto.
+   
+   apply (NREC_inv _ _ _ _ zero_typ) in H1; trivial.
+   apply (NREC_inv _ _ _ _ zero_typ) in H2; trivial.
+   destruct H1 as (?, (?, (?, ?))). rewrite (H4 (reflexivity zero)).
+   destruct H2 as (?, (?, (?, ?))). rewrite (H7 (reflexivity zero)).
+   reflexivity.
+   
+   apply (NREC_inv _ _ _ _ (succ_typ _ H1)) in H3; trivial.
+   apply (NREC_inv _ _ _ _ (succ_typ _ H1)) in H4; trivial.
+   destruct H3 as (?, (?, (?, ?))). 
+   destruct (H7 n0 H1 (reflexivity (succ n0))). rewrite H9. 
+   destruct H4 as (?, (?, (?, ?))). 
+   destruct (H12 n0 H1 (reflexivity (succ n0))). rewrite H14.
+   apply H0. reflexivity. auto.
+Qed.
+
+Lemma uchoice_NREC_0 : forall f g, uchoice_pred (NREC f g zero).
+split; try split; intros.
+ unfold NREC; intros. rewrite <- H. apply H0; auto.
+ 
+ exists f. unfold NREC; intros; auto.
+
+ cut (zero == zero); try reflexivity.
+  pattern zero at 2, x'; apply H0; intros.
+   repeat red; intros. rewrite H1. rewrite H2. auto.
+
+   revert H1; pattern zero at 2, x; apply H; intros.
+    repeat red; intros. rewrite H1, H2. auto.
+
+    reflexivity.
+
+    symmetry in H2. apply discr in H2; contradiction.
+
+    symmetry in H2. apply discr in H2; contradiction.
+Qed.
+
+  
+
+Definition NATREC f g n := uchoice (NREC f g n).
+
+Instance NATREC_morph : 
+  Proper (eq_set ==> (eq_set ==> eq_set ==> eq_set) ==> eq_set ==> eq_set) NATREC.
+repeat red; intros. unfold NATREC, NREC; intros. 
+apply uchoice_morph_raw; repeat red; intros.
+apply fa_morph; intros. 
+apply fa_morph; intros. rewrite H.
+apply fa_morph; intros. split; intros.
+ rewrite <- H2. rewrite <- H1. apply H3. intros. 
+ setoid_replace (x0 m t) with (y0 m t). 
+  auto. 
+  apply H0; reflexivity.
+
+ rewrite H2. rewrite H1. apply H3. intros.
+ setoid_replace (y0 m t) with (x0 m t).
+  auto.
+  symmetry. apply H0; reflexivity.
+Qed.
+
+Lemma NATREC_0 : forall f g, NATREC f g zero == f.
+unfold NATREC; intros.
+symmetry. apply uchoice_ext. 
+ apply uchoice_NREC_0.
+ 
+ unfold NREC; intros; auto.
+Qed.
+
+Lemma NATREC_Succ : forall f g n, morph2 g -> n \in N ->
+  NATREC f g (succ n) == g n (NATREC f g n).
+intros. elim H0 using N_ind; intros.
+ rewrite <- H2; auto.
+ 
+ rewrite NATREC_0. unfold NATREC. symmetry. apply uchoice_ext.
+ apply NREC_choice. 
+  apply succ_typ; apply zero_typ.
+  assumption.
+
+  unfold NREC; intros. apply H3; assumption.
+
+ rewrite H2. unfold NATREC at 1. symmetry. apply uchoice_ext.
+  apply NREC_choice; trivial. repeat apply succ_typ; auto.
+  
+  repeat red; intros. apply H5. apply H5.
+  revert P H3 H4 H5. change (NREC f g n0 (NATREC f g n0)).
+  unfold NATREC; apply uchoice_def. apply NREC_choice; auto.
+Qed.
+
+Definition NatRec (f g n:term) : term.
+left; exists (fun i => NATREC (int f i) 
+  (fun m t => app (app (int g i) m) t) (int n i)).
+repeat red; intros. apply NATREC_morph. 
+ rewrite H; reflexivity.
+ 
+ repeat red; intros. rewrite H, H0, H1. reflexivity.
+
+ rewrite H; reflexivity.
+Defined.
+   
 
 Lemma typ_Nrect : forall e n f g P,
   typ e n T ->
-  typ e P (Prod T prop) -> 
+  typ e P (Prod T kind) -> 
   typ e f (App P Zero) ->
   typ e g (Prod T (Prod (App (lift 1 P) (Ref 0))
-              (App (lift 2 P) (App Succ (Ref 1))))) ->
+              (App (lift 2 P) ( Succ (Ref 1))))) ->
   typ e (NatRec f g n) (App P n).
-do 2 red; simpl; intros.
-red in H. simpl in H.
-  assert (int n i == empty). apply H in H3. apply (singl_elim _ _ H3).
-  rewrite H4. apply H1. apply H3.
+do 2 red. simpl. intros.
+red in H; specialize H with (1:=H3).
+red in H0; specialize H0 with (1:=H3).
+red in H1; specialize H1 with (1:=H3).
+red in H2; specialize H2 with (1:=H3).
+simpl in *.
+replace (fun k0 : nat => i k0) with i in *; trivial.
+set (c := int n i) in *; clearbody c.
+set (f0 := int f i) in *; clearbody f0.
+set (fS := int g i) in *; clearbody fS.
+
+elim H using N_ind; intros. 
+ revert H6. apply in_set_morph.
+  apply NATREC_morph.
+   reflexivity.
+   do 2 red; intros. rewrite H7. rewrite H6. reflexivity.
+   symmetry; assumption.
+  rewrite H5; reflexivity.
+
+ rewrite NATREC_0. apply H1.
+ 
+ rewrite NATREC_Succ; auto.
+  refine (let H6 := prod_elim _ _ _ _ _ H2 H4 in _).
+   red; intros. apply prod_ext.
+    apply app_ext; try assumption.
+     apply int_morph; try reflexivity.
+      do 2 red; intros. rewrite H7; reflexivity.
+   
+    red; intros. apply app_ext.
+     apply int_morph; try reflexivity.
+      do 2 red; intros. apply V.cons_morph; try assumption.
+       do 2 red; intros. rewrite H7; reflexivity.
+
+     rewrite H7; reflexivity.
+
+  simpl in H6. clear H2. 
+  replace (fun k : nat => V.cons n0 i k) with (V.cons n0 i) in *; trivial.
+  refine (let H7 := prod_elim _ _ _ _ _ H6 _ in _).
+   do 2 red; intros. apply app_ext; try reflexivity.
+    apply int_morph; try reflexivity.
+     do 2 red; intros. rewrite H7; reflexivity.
+   
+   rewrite simpl_int_lift1. apply H5.
+
+  simpl in H7. revert H7. apply in_set_morph; try reflexivity.
+  set (fS' := fun n y :set => app (app fS n) y) in |-*.
+   apply app_ext; try reflexivity.
+    replace (fun k : nat => V.cons (NATREC f0 fS' n0) (V.cons n0 i) k) 
+    with (V.cons (NATREC f0 fS' n0) (V.cons n0 i)); trivial.
+    rewrite simpl_int_lift. symmetry; apply simpl_int_lift1.
+
+  do 3 red; intros. rewrite H6, H7; reflexivity.
 Qed. 
 
+Definition Add : term -> term -> term.
+intros m n; left; exists (fun i => NATREC (int m i) (fun _ => succ) (int n i)).
+do 2 red; intros. apply NATREC_morph; try rewrite H; try reflexivity.
+ do 2 red; intros. rewrite H1; reflexivity.
+Defined.
 
-Lemma all_conv_allowed : forall e M M',
-  typ e M T ->
-  typ e M' T ->
-  eq_typ e M M'.
-do 2 red; intros.
-  assert (int M i == empty). red in H; simpl in H. 
-    apply singl_elim. apply H. apply H1.
-  assert (int M' i == empty). red in H0; simpl in H0; 
-    apply singl_elim; apply H0; apply H1.
-  rewrite H2; rewrite H3; reflexivity.
+Lemma typ_Add : forall e m n, typ e m T -> typ e n T -> 
+  typ e (Add m n) T.
+Proof.
+do 2 red; simpl; intros.
+replace (fun k : nat => i k) with i; trivial.
+do 2 red in H0; simpl in H0; specialize H0 with (1:=H1).
+do 2 red in H; simpl in H; specialize H with (1:=H1).
+elim H0 using N_ind; intros.
+ revert H4; apply in_set_morph; try reflexivity.
+  apply NATREC_morph; try reflexivity; try symmetry; trivial.
+   do 2 red; intros; rewrite H5; reflexivity.
+   
+ rewrite NATREC_0; trivial.
+
+ rewrite NATREC_Succ; trivial.
+  apply succ_typ; trivial.
+    
+  do 3 red; intros. rewrite H5; reflexivity.
 Qed.
+
+(*Definition Add : term.
+left; exists (fun i => lam N (fun m => lam N (fun n => NATREC m (fun _ => succ) n))).
+do 2 red; intros. apply lam_ext; try reflexivity.
+ do 2 red; intros. apply lam_ext; try reflexivity.
+  do 2 red; intros. apply NATREC_morph; trivial.
+   do 2 red; intros. rewrite H5; reflexivity.
+Defined.
+
+Lemma typ_Add : forall e, typ e Add (Prod T (Prod (lift 1 T) (lift 2 T))).
+Proof.
+do 2 red; simpl; intros.
+apply prod_intro.
+ do 2 red; intros; apply lam_ext; try reflexivity.
+  do 2 red; intros. apply NATREC_morph; trivial.
+   do 2 red; intros. rewrite H5; reflexivity.
+
+ do 2 red; intros; try reflexivity.
+
+ intros. apply prod_intro.
+  do 2 red; intros; try reflexivity.
+   apply NATREC_morph; try reflexivity; trivial.
+    do 2 red; intros; rewrite H4; reflexivity.
+
+  do 2 red; intros; reflexivity.
+
+  intros. elim H1 using N_ind; intros.
+   revert H4; apply in_set_morph; try reflexivity.
+    apply NATREC_morph; try reflexivity; try symmetry; trivial.
+     do 2 red; intros; rewrite H5; reflexivity.
+   
+   rewrite NATREC_0; trivial.
+
+   rewrite NATREC_Succ; trivial.
+    apply succ_typ; trivial.
+    
+    do 3 red; intros. rewrite H5; reflexivity.
+
+Qed.*)
+   
+
+(*Inductive is_clsd_foterm : term -> Prop := 
+| const : is_clsd_foterm Zero  
+| suc : forall x, is_clsd_foterm x -> is_clsd_foterm (App Succ x).
+
+Lemma clsd_foterm_typ : forall t e, is_clsd_foterm t -> typ e t T.
+Proof.
+induction 1 as [|t H IH]; do 2 red; simpl; intros i He.
+ apply zero_typ.
+ 
+ do 2 red in IH; specialize IH with (1 := He); simpl in *.
+ rewrite beta_eq.
+  apply succ_typ; apply IH.
+
+  do 2 red; intros. rewrite H1; reflexivity.
+
+  apply IH.
+Qed.*)
+
+Inductive is_foterm : term -> Prop :=
+| T_var : forall n, is_foterm n
+| T_0   : is_foterm Zero
+| T_S   : forall n, is_foterm n -> is_foterm (Succ n)
+| T_Add : forall m n, is_foterm m -> is_foterm n -> is_foterm (Add m n).
+
+Lemma foterm_typ : forall t e, is_foterm t -> (forall n, typ e n T) -> typ e t T.
+Proof.
+induction 1 as [ | |t H IH | u v  H1 IH1 H2 IH2]; do 2 red; simpl; intros.
+ apply H. apply H0.
+
+ apply zero_typ.
+
+ specialize IH with (1:=H0). 
+ do 2 red in IH; specialize IH with (1 := H1); simpl in *.
+ apply succ_typ; apply IH.
+  
+ specialize IH1 with (1:=H).
+ specialize IH2 with (1:=H).
+ refine (let Hta := typ_Add in _); clearbody Hta.
+ specialize Hta with (1:=IH1) (2:=IH2).
+ do 2 red in Hta; simpl in Hta; specialize Hta with (1:=H0).
+ apply Hta.
+Qed.
+
+Lemma discr_term : forall n, ~ eq_term Zero (Add n (Succ Zero)).
+red; intros. red in H; simpl in H; red in H.
+refine (let v := (fun _ => empty) : val in _); clearbody v. 
+assert (eq_val v v); try reflexivity. 
+ specialize H with (1:=H0). rewrite NATREC_Succ in H.
+  rewrite NATREC_0 in H. symmetry in H; apply discr in H; trivial.
+
+ do 3 red; intros. rewrite H2; reflexivity.
+
+ apply zero_typ.
+Qed.
+
+Lemma Succ_inj : forall x y, x <> None -> y <> None ->
+ (forall v, int x v \in N /\ int y v \in N) -> 
+  eq_term (Succ x) (Succ y) -> eq_term x y.
+intros x y HxN HyN H HSucc; destruct x; destruct y; simpl; trivial.
+ repeat red in HSucc; repeat red; simpl in *; intros.
+ destruct H with (v:=x) as (HNx, _).
+ destruct H with (v:=y) as (_, HNy).
+ specialize HSucc with (1 := H0); apply succ_inj.
+  apply HNx.
+  apply HNy.
+  apply HSucc.
+
+ elim HyN; reflexivity.
+ 
+ elim HxN; reflexivity.
+Qed.
+
+Lemma eq_props_2 : props == succ (succ zero).
+unfold props; unfold ZFcoc.props. 
+replace prf_trm with empty; trivial.
+replace zero with empty; trivial. unfold succ.
+assert (union2 empty (singl empty) == singl empty).
+ apply eq_intro; intros.
+  apply union2_elim in H; destruct H; trivial.
+   apply empty_ax in H; contradiction.
+
+   apply union2_intro2; trivial.
+rewrite H. 
+assert (union2 (singl empty) (singl (singl empty)) == pair empty (singl empty)).
+ apply eq_intro; intros.
+  apply union2_elim in H0; destruct H0; apply singl_elim in H0; 
+   rewrite pair_ax; [left | right]; trivial.
+  
+ apply pair_elim in H0; destruct H0.
+  apply union2_intro1; apply singl_intro_eq; apply H0.
+
+  apply union2_intro2; apply singl_intro_eq; apply H0.
+rewrite H0. clear H H0.
+symmetry; apply power_ext; intros.
+ admit.
+
+ apply pair_elim in H; destruct H; rewrite H in H0; trivial.
+  apply empty_ax in H0; contradiction.
+Qed.
+ 
+ 
+ 
+   
+   
+   
+
+   
+ 
+Lemma Add_0 : forall n, n <> None -> eq_term (Add n Zero) n.
+destruct n; simpl; intros.
+ do 2 red; intros; rewrite NATREC_0.
+ replace (fun k : nat => x k) with x; trivial.
+ destruct s; simpl; rewrite H0; reflexivity.
+
+ apply H; reflexivity.
+Qed.
+
+Lemma Add_ass : forall x y, x <> None -> y <> None -> (forall i, int y i \in N) ->
+ eq_term (Add (Add x y) (Succ Zero)) (Add x (Add y (Succ Zero))).
+simpl; red; intros. 
+replace (fun k : nat => x0 k) with x0; trivial.
+replace (fun k : nat => y0 k) with y0; trivial.
+assert (morph2 (fun _ : set => succ)).
+ do 3 red; intros. rewrite H4; reflexivity.
+assert (zero \in N). apply zero_typ.
+rewrite (NATREC_Succ _ _ _ H3 H4). rewrite NATREC_0.
+rewrite (NATREC_Succ _ _ _ H3 H4). rewrite NATREC_0. 
+rewrite (NATREC_Succ _ _ _ H3 (H1 y0)).
+do 3 red in H3. apply (H3 zero zero (reflexivity zero)).
+apply NATREC_morph.
+ rewrite H2; reflexivity.
+
+ do 2 red; intros. rewrite H6; reflexivity.
+
+ rewrite H2; reflexivity.
+Qed.
+
+Lemma foformula : forall P n, is_foterm n ->
+  (forall k i, int k i \in N) ->
+  P Zero ->
+  (forall m, P m -> P (Succ m)) -> 
+  P n. 
+
+
+
+ 
+
+
 
 
 
