TermCCUT.v
@@ -1,0 +1,958 @@
+
+Require Export Arith.
+Require Export Compare_dec.
+Require Export Relations.
+Require Export List.
+
+Hint Resolve t_step rt_step rt_refl: core.
+Hint Unfold transp: core.
+
+Section Termes.
+
+  Inductive sort : Set :=
+    | kind : nat -> sort
+    | prop : sort.
+
+  Inductive term : Set :=
+    | Srt : sort -> term
+    | Zero : term
+    | Succ : term -> term
+    | Add : term -> term -> term
+    | Ref : nat -> term
+    | Abs : term -> term -> term
+    | App : term -> term -> term
+    | Prod : term -> term -> term
+    | Elim : term -> term -> term -> term -> term.
+
+  Fixpoint lift_rec (n : nat) (t : term) (k : nat) {struct t} : term :=
+    match t with
+    | Srt s => Srt s
+    | Zero => Zero
+    | Succ m => Succ (lift_rec n m k)
+    | Add p q => Add (lift_rec n p k) (lift_rec n q k)
+    | Ref i =>
+        match le_gt_dec k i with
+        | left _ => Ref (n + i)
+        | right _ => Ref i
+        end
+    | Abs T M => Abs (lift_rec n T k) (lift_rec n M (S k))
+    | App u v => App (lift_rec n u k) (lift_rec n v k)
+    | Prod A B => Prod (lift_rec n A k) (lift_rec n B (S k))
+    | Elim Q f g m => 
+        Elim (lift_rec n Q k) (lift_rec n f k) (lift_rec n g k) (lift_rec n m k)
+    end.
+
+  Definition lift n t := lift_rec n t 0.
+
+  Fixpoint subst_rec (N M : term) (k : nat) {struct M} : term :=
+    match M with
+    | Srt s => Srt s
+    | Zero => Zero
+    | Succ t => Succ (subst_rec N t k)
+    | Add p q => Add (subst_rec N p k) (subst_rec N q k)
+    | Ref i =>
+        match lt_eq_lt_dec k i with
+        | inleft (left _) => Ref (pred i)
+        | inleft (right _) => lift k N
+        | inright _ => Ref i
+        end
+    | Abs A B => Abs (subst_rec N A k) (subst_rec N B (S k))
+    | App u v => App (subst_rec N u k) (subst_rec N v k)
+    | Prod T U => Prod (subst_rec N T k) (subst_rec N U (S k))
+    | Elim Q f g m => 
+        Elim (subst_rec N Q k) (subst_rec N f k) (subst_rec N g k) (subst_rec N m k)
+    end.
+
+  Definition subst N M := subst_rec N M 0.
+
+
+  Inductive subterm : term -> term -> Prop :=
+    | sbtrm_succ : forall A, subterm A (Succ A)
+    | sbtrm_add_l : forall A B, subterm A (Add A B)
+    | sbtrm_add_r : forall A B, subterm B (Add A B)
+    | sbtrm_abs_l : forall A B, subterm A (Abs A B)
+    | sbtrm_abs_r : forall A B, subterm B (Abs A B)
+    | sbtrm_app_l : forall A B, subterm A (App A B)
+    | sbtrm_app_r : forall A B, subterm B (App A B)
+    | sbtrm_prod_l : forall A B, subterm A (Prod A B)
+    | sbtrm_prod_r : forall A B, subterm B (Prod A B)
+    | sbtrm_elim_Q : forall Q f g n, subterm Q (Elim Q f g n)
+    | sbtrm_elim_f : forall Q f g n, subterm f (Elim Q f g n)
+    | sbtrm_elim_g : forall Q f g n, subterm g (Elim Q f g n)
+    | sbtrm_elim_n : forall Q f g n, subterm n (Elim Q f g n).
+
+  Inductive mem_sort (s : sort) : term -> Prop :=
+    | mem_eq : mem_sort s (Srt s)
+    | mem_prod_l : forall u v, mem_sort s u -> mem_sort s (Prod u v)
+    | mem_prod_r : forall u v, mem_sort s v -> mem_sort s (Prod u v)
+    | mem_abs_l : forall u v, mem_sort s u -> mem_sort s (Abs u v)
+    | mem_abs_r : forall u v, mem_sort s v -> mem_sort s (Abs u v)
+    | mem_app_l : forall u v, mem_sort s u -> mem_sort s (App u v)
+    | mem_app_r : forall u v, mem_sort s v -> mem_sort s (App u v).
+
+  Inductive foterm : term -> Prop := 
+    | Val : forall n, foterm (Ref n)
+    | Cst_0 : foterm Zero
+    | Cst_S : forall m, foterm m -> foterm (Succ m)
+    | Df_Add : forall m n, foterm m -> foterm n -> foterm (Add m n).
+
+  Definition substitution := list term.
+
+  Definition app_subst M s := fold_left (fun m n => subst n m) s M.
+
+End Termes.
+
+  Hint Constructors subterm: coc.
+  Hint Constructors mem_sort: coc.
+
+Section Beta_Reduction.
+
+  Inductive red1 : term -> term -> Prop :=
+    | beta : forall M N T, red1 (App (Abs T M) N) (subst N M)
+    | abs_red_l :
+        forall M M', red1 M M' -> forall N, red1 (Abs M N) (Abs M' N)
+    | abs_red_r :
+        forall M M', red1 M M' -> forall N, red1 (Abs N M) (Abs N M')
+    | app_red_l :
+        forall M1 N1, red1 M1 N1 -> forall M2, red1 (App M1 M2) (App N1 M2)
+    | app_red_r :
+        forall M2 N2, red1 M2 N2 -> forall M1, red1 (App M1 M2) (App M1 N2)
+    | prod_red_l :
+        forall M1 N1, red1 M1 N1 -> forall M2, red1 (Prod M1 M2) (Prod N1 M2)
+    | prod_red_r :
+        forall M2 N2, red1 M2 N2 -> forall M1, red1 (Prod M1 M2) (Prod M1 N2).
+
+  Inductive red (M : term) : term -> Prop :=
+    | refl_red : red M M
+    | trans_red : forall P N, red M P -> red1 P N -> red M N.
+
+  Inductive conv (M : term) : term -> Prop :=
+    | refl_conv : conv M M
+    | trans_conv_red : forall P N, conv M P -> red1 P N -> conv M N
+    | trans_conv_exp : forall P N, conv M P -> red1 N P -> conv M N.
+
+  Inductive par_red1 : term -> term -> Prop :=
+    | par_beta :
+        forall M M' N N' T,
+        par_red1 M M' ->
+        par_red1 N N' -> par_red1 (App (Abs T M) N) (subst N' M')
+    | sort_par_red : forall s, par_red1 (Srt s) (Srt s)
+    | ref_par_red : forall n, par_red1 (Ref n) (Ref n)
+    | abs_par_red :
+        forall M M' T T',
+        par_red1 M M' -> par_red1 T T' -> par_red1 (Abs T M) (Abs T' M')
+    | app_par_red :
+        forall M M' N N',
+        par_red1 M M' -> par_red1 N N' -> par_red1 (App M N) (App M' N')
+    | prod_par_red :
+        forall M M' N N',
+        par_red1 M M' -> par_red1 N N' -> par_red1 (Prod M N) (Prod M' N').
+
+  Definition par_red := clos_trans term par_red1.
+
+End Beta_Reduction.
+
+
+  Hint Constructors red1: coc.
+  Hint Constructors par_red1: coc.
+  Hint Resolve refl_red refl_conv: coc.
+  Hint Unfold par_red: coc.
+
+
+Section Normalisation_Forte.
+
+  Definition normal t := forall u, ~ red1 t u.
+
+  Definition sn := Acc (transp _ red1).
+
+End Normalisation_Forte.
+
+  Hint Unfold sn: coc.
+ 
+
+  Lemma inv_lift_sort :  forall s n t k, lift_rec n t k = Srt s -> t = Srt s.
+intros.
+destruct t; try  discriminate H.
+ auto.
+ unfold lift_rec in H.
+   destruct (le_gt_dec k n0);  discriminate H.
+Qed.
+
+  Lemma inv_subst_sort :
+    forall s x t k, subst_rec x t k = Srt s -> t = Srt s \/ x = Srt s.
+intros.
+destruct t; try  discriminate H.
+ auto.
+ unfold subst_rec in H.
+   destruct (lt_eq_lt_dec k n) as [[fv| eqv]| bv]; try  discriminate H.
+   right.
+   unfold lift in H.
+   apply inv_lift_sort with (1 := H).
+Qed.
+
+
+  Lemma lift_ref_ge :
+   forall k n p, p <= n -> lift_rec k (Ref n) p = Ref (k + n).
+intros; simpl in |- *.
+elim (le_gt_dec p n); auto with arith.
+intro; absurd (p <= n); auto with arith.
+Qed.
+
+
+  Lemma lift_ref_lt : forall k n p, p > n -> lift_rec k (Ref n) p = Ref n.
+intros; simpl in |- *.
+elim (le_gt_dec p n); auto with arith.
+intro; absurd (p <= n); auto with arith.
+Qed.
+
+
+  Lemma subst_ref_lt : forall u n k, k > n -> subst_rec u (Ref n) k = Ref n.
+simpl in |- *; intros.
+elim (lt_eq_lt_dec k n); intros; auto with arith.
+elim a; intros.
+absurd (k <= n); auto with arith.
+
+inversion_clear b in H.
+elim gt_irrefl with n; auto with arith.
+Qed.
+
+
+  Lemma subst_ref_gt :
+   forall u n k, n > k -> subst_rec u (Ref n) k = Ref (pred n).
+simpl in |- *; intros.
+elim (lt_eq_lt_dec k n); intros.
+elim a; intros; auto with arith.
+inversion_clear b in H.
+elim gt_irrefl with n; auto with arith.
+
+absurd (k <= n); auto with arith.
+Qed.
+
+
+  Lemma subst_ref_eq : forall u n, subst_rec u (Ref n) n = lift n u.
+intros; simpl in |- *.
+elim (lt_eq_lt_dec n n); intros.
+elim a; intros; auto with coc.
+elim lt_irrefl with n; auto with coc.
+
+elim gt_irrefl with n; auto with coc.
+Qed.
+
+
+
+  Lemma lift_rec0 : forall M k, lift_rec 0 M k = M.
+simple induction M; simpl in |- *; intros; auto with coc.
+elim (le_gt_dec k n); auto with coc.
+
+rewrite H; rewrite H0; auto with coc.
+
+rewrite H; rewrite H0; auto with coc.
+
+rewrite H; rewrite H0; auto with coc.
+Qed.
+
+
+  Lemma lift0 : forall M, lift 0 M = M.
+intros; unfold lift in |- *.
+apply lift_rec0; auto with coc.
+Qed.
+
+
+  Lemma simpl_lift_rec :
+   forall M n k p i,
+   i <= k + n ->
+   k <= i -> lift_rec p (lift_rec n M k) i = lift_rec (p + n) M k.
+simple induction M; simpl in |- *; intros; auto with coc.
+elim (le_gt_dec k n); intros.
+rewrite lift_ref_ge; auto with coc.
+rewrite plus_assoc; auto with coc.
+
+rewrite plus_comm.
+apply le_trans with (k + n0); auto with arith.
+
+rewrite lift_ref_lt; auto with arith.
+apply le_gt_trans with k; auto with arith.
+
+rewrite H; auto with arith; rewrite H0; simpl in |- *; auto with arith.
+
+rewrite H; auto with arith; rewrite H0; simpl in |- *; auto with arith.
+
+rewrite H; auto with arith; rewrite H0; simpl in |- *; auto with arith.
+Qed.
+
+
+  Lemma simpl_lift : forall M n, lift (S n) M = lift 1 (lift n M).
+intros; unfold lift in |- *.
+rewrite simpl_lift_rec; auto with arith.
+Qed.
+
+
+  Lemma permute_lift_rec :
+   forall M n k p i,
+   i <= k ->
+   lift_rec p (lift_rec n M k) i = lift_rec n (lift_rec p M i) (p + k).
+simple induction M; simpl in |- *; intros; auto with coc.
+elim (le_gt_dec k n); elim (le_gt_dec i n); intros.
+rewrite lift_ref_ge; auto with arith.
+rewrite lift_ref_ge; auto with arith.
+elim plus_assoc_reverse with p n0 n.
+elim plus_assoc_reverse with n0 p n.
+elim plus_comm with p n0; auto with arith.
+
+apply le_trans with n; auto with arith.
+
+absurd (i <= n); auto with arith.
+apply le_trans with k; auto with arith.
+
+rewrite lift_ref_ge; auto with arith.
+rewrite lift_ref_lt; auto with arith.
+
+rewrite lift_ref_lt; auto with arith.
+rewrite lift_ref_lt; auto with arith.
+apply le_gt_trans with k; auto with arith.
+
+rewrite H; auto with arith; rewrite H0; auto with arith.
+rewrite plus_n_Sm; auto with arith.
+
+rewrite H; auto with arith; rewrite H0; auto with arith.
+
+rewrite H; auto with arith; rewrite H0; auto with arith.
+rewrite plus_n_Sm; auto with arith.
+Qed.
+
+
+  Lemma permute_lift :
+   forall M k, lift 1 (lift_rec 1 M k) = lift_rec 1 (lift 1 M) (S k).
+intros.
+change (lift_rec 1 (lift_rec 1 M k) 0 = lift_rec 1 (lift_rec 1 M 0) (1 + k))
+ in |- *.
+apply permute_lift_rec; auto with arith.
+Qed.
+
+
+  Lemma simpl_subst_rec :
+   forall N M n p k,
+   p <= n + k ->
+   k <= p -> subst_rec N (lift_rec (S n) M k) p = lift_rec n M k.
+simple induction M; simpl in |- *; intros; auto with arith.
+elim (le_gt_dec k n); intros.
+rewrite subst_ref_gt; auto with arith.
+red in |- *; red in |- *.
+apply le_trans with (S (n0 + k)); auto with arith.
+
+rewrite subst_ref_lt; auto with arith.
+apply le_gt_trans with k; auto with arith.
+
+rewrite H; auto with arith; rewrite H0; auto with arith.
+elim plus_n_Sm with n k; auto with arith.
+
+rewrite H; auto with arith; rewrite H0; auto with arith.
+
+rewrite H; auto with arith; rewrite H0; auto with arith.
+elim plus_n_Sm with n k; auto with arith.
+Qed.
+
+
+  Lemma simpl_subst :
+   forall N M n p, p <= n -> subst_rec N (lift (S n) M) p = lift n M.
+intros; unfold lift in |- *.
+apply simpl_subst_rec; auto with arith.
+Qed.
+
+
+  Lemma commut_lift_subst_rec :
+   forall M N n p k,
+   k <= p ->
+   lift_rec n (subst_rec N M p) k = subst_rec N (lift_rec n M k) (n + p).
+simple induction M; intros; auto with arith.
+unfold subst_rec at 1, lift_rec at 2 in |- *.
+elim (lt_eq_lt_dec p n); elim (le_gt_dec k n); intros.
+elim a0.
+case n; intros.
+inversion_clear a1.
+
+unfold pred in |- *.
+rewrite lift_ref_ge; auto with arith.
+rewrite subst_ref_gt; auto with arith.
+elim plus_n_Sm with n0 n1.
+auto with arith.
+
+apply le_trans with p; auto with arith.
+
+simple induction 1.
+rewrite subst_ref_eq.
+unfold lift in |- *.
+rewrite simpl_lift_rec; auto with arith.
+
+absurd (k <= n); auto with arith.
+apply le_trans with p; auto with arith.
+elim a; auto with arith.
+simple induction 1; auto with arith.
+
+rewrite lift_ref_ge; auto with arith.
+rewrite subst_ref_lt; auto with arith.
+
+rewrite lift_ref_lt; auto with arith.
+rewrite subst_ref_lt; auto with arith.
+apply le_gt_trans with p; auto with arith.
+
+simpl in |- *.
+rewrite plus_n_Sm.
+rewrite H; auto with arith; rewrite H0; auto with arith.
+
+simpl in |- *; rewrite H; auto with arith; rewrite H0; auto with arith.
+
+simpl in |- *; rewrite plus_n_Sm.
+rewrite H; auto with arith; rewrite H0; auto with arith.
+Qed.
+
+
+  Lemma commut_lift_subst :
+   forall M N k, subst_rec N (lift 1 M) (S k) = lift 1 (subst_rec N M k).
+intros; unfold lift in |- *.
+rewrite commut_lift_subst_rec; auto with arith.
+Qed.
+
+
+  Lemma distr_lift_subst_rec :
+   forall M N n p k,
+   lift_rec n (subst_rec N M p) (p + k) =
+   subst_rec (lift_rec n N k) (lift_rec n M (S (p + k))) p.
+simple induction M; intros; auto with arith.
+unfold subst_rec at 1 in |- *.
+elim (lt_eq_lt_dec p n); intro.
+elim a.
+case n; intros.
+inversion_clear a0.
+
+unfold pred, lift_rec at 1 in |- *.
+elim (le_gt_dec (p + k) n1); intro.
+rewrite lift_ref_ge; auto with arith.
+elim plus_n_Sm with n0 n1.
+rewrite subst_ref_gt; auto with arith.
+red in |- *; red in |- *; apply le_n_S.
+apply le_trans with (n0 + (p + k)); auto with arith.
+apply le_trans with (p + k); auto with arith.
+
+rewrite lift_ref_lt; auto with arith.
+rewrite subst_ref_gt; auto with arith.
+
+simple induction 1.
+unfold lift in |- *.
+rewrite <- permute_lift_rec; auto with arith.
+rewrite lift_ref_lt; auto with arith.
+rewrite subst_ref_eq; auto with arith.
+
+rewrite lift_ref_lt; auto with arith.
+rewrite lift_ref_lt; auto with arith.
+rewrite subst_ref_lt; auto with arith.
+
+simpl in |- *; replace (S (p + k)) with (S p + k); auto with arith.
+rewrite H; rewrite H0; auto with arith.
+
+simpl in |- *; rewrite H; rewrite H0; auto with arith.
+
+simpl in |- *; replace (S (p + k)) with (S p + k); auto with arith.
+rewrite H; rewrite H0; auto with arith.
+Qed.
+
+
+  Lemma distr_lift_subst :
+   forall M N n k,
+   lift_rec n (subst N M) k = subst (lift_rec n N k) (lift_rec n M (S k)).
+intros; unfold subst in |- *.
+pattern k at 1 3 in |- *.
+replace k with (0 + k); auto with arith.
+apply distr_lift_subst_rec.
+Qed.
+
+
+  Lemma distr_subst_rec :
+   forall M N P n p,
+   subst_rec P (subst_rec N M p) (p + n) =
+   subst_rec (subst_rec P N n) (subst_rec P M (S (p + n))) p.
+simple induction M; auto with arith; intros.
+unfold subst_rec at 2 in |- *.
+elim (lt_eq_lt_dec p n); intro.
+elim a.
+case n; intros.
+inversion_clear a0.
+
+unfold pred, subst_rec at 1 in |- *.
+elim (lt_eq_lt_dec (p + n0) n1); intro.
+elim a1.
+case n1; intros.
+inversion_clear a2.
+
+rewrite subst_ref_gt; auto with arith.
+rewrite subst_ref_gt; auto with arith.
+apply gt_le_trans with (p + n0); auto with arith.
+
+simple induction 1.
+rewrite subst_ref_eq; auto with arith.
+rewrite simpl_subst; auto with arith.
+
+rewrite subst_ref_lt; auto with arith.
+rewrite subst_ref_gt; auto with arith.
+
+simple induction 1.
+rewrite subst_ref_lt; auto with arith.
+rewrite subst_ref_eq.
+unfold lift in |- *.
+rewrite commut_lift_subst_rec; auto with arith.
+
+do 3 (rewrite subst_ref_lt; auto with arith).
+
+simpl in |- *; replace (S (p + n)) with (S p + n); auto with arith.
+rewrite H; auto with arith; rewrite H0; auto with arith.
+
+simpl in |- *; rewrite H; rewrite H0; auto with arith.
+
+simpl in |- *; replace (S (p + n)) with (S p + n); auto with arith.
+rewrite H; rewrite H0; auto with arith.
+Qed.
+
+
+  Lemma distr_subst :
+   forall P N M k,
+   subst_rec P (subst N M) k = subst (subst_rec P N k) (subst_rec P M (S k)).
+intros; unfold subst in |- *.
+pattern k at 1 3 in |- *.
+replace k with (0 + k); auto with arith.
+apply distr_subst_rec.
+Qed.
+
+
+
+  Lemma one_step_red : forall M N, red1 M N -> red M N.
+intros.
+apply trans_red with M; auto with coc.
+Qed.
+
+  Hint Resolve one_step_red: coc.
+
+
+  Lemma red1_red_ind :
+   forall N P,
+   (P:term -> Prop) N ->
+   (forall M R, red1 M R -> red R N -> P R -> P M) ->
+   forall M, red M N -> P M.
+cut
+ (forall M N,
+  red M N ->
+  forall P : term -> Prop,
+  P N -> (forall M R, red1 M R -> red R N -> P R -> P M) -> P M).
+intros.
+apply (H M N); auto with coc.
+
+simple induction 1; intros; auto with coc.
+apply H1; auto with coc.
+apply H4 with N0; auto with coc.
+
+intros.
+apply H4 with R; auto with coc.
+apply trans_red with P; auto with coc.
+Qed.
+
+
+  Lemma trans_red_red : forall M N P, red M N -> red N P -> red M P.
+intros.
+generalize H0 M H.
+simple induction 1; auto with coc.
+intros.
+apply trans_red with P0; auto with coc.
+Qed.
+ 
+
+  Lemma red_red_app :
+   forall u u0 v v0, red u u0 -> red v v0 -> red (App u v) (App u0 v0).
+simple induction 1.
+simple induction 1; intros; auto with coc.
+apply trans_red with (App u P); auto with coc.
+
+intros.
+apply trans_red with (App P v0); auto with coc.
+Qed.
+
+
+  Lemma red_red_abs :
+   forall u u0 v v0, red u u0 -> red v v0 -> red (Abs u v) (Abs u0 v0).
+simple induction 1.
+simple induction 1; intros; auto with coc.
+apply trans_red with (Abs u P); auto with coc.
+
+intros.
+apply trans_red with (Abs P v0); auto with coc.
+Qed.
+
+
+  Lemma red_red_prod :
+   forall u u0 v v0, red u u0 -> red v v0 -> red (Prod u v) (Prod u0 v0).
+simple induction 1.
+simple induction 1; intros; auto with coc.
+apply trans_red with (Prod u P); auto with coc.
+
+intros.
+apply trans_red with (Prod P v0); auto with coc.
+Qed.
+
+  Hint Resolve red_red_app red_red_abs red_red_prod: coc.
+
+
+
+  Lemma red1_lift :
+   forall n u v, red1 u v -> forall k, red1 (lift_rec n u k) (lift_rec n v k).
+simple induction 1; simpl in |- *; intros; auto with coc.
+rewrite distr_lift_subst; auto with coc.
+Qed.
+
+  Hint Resolve red1_lift: coc.
+
+
+  Lemma red1_subst_r :
+   forall a t u,
+   red1 t u -> forall k, red1 (subst_rec a t k) (subst_rec a u k).
+simple induction 1; simpl in |- *; intros; auto with coc.
+rewrite distr_subst; auto with coc.
+Qed.
+
+
+  Lemma red1_subst_l :
+   forall t u,
+   red1 t u -> forall a k, red (subst_rec t a k) (subst_rec u a k).
+simple induction a; simpl in |- *; auto with coc.
+intros.
+elim (lt_eq_lt_dec k n); intros; auto with coc.
+elim a0; auto with coc.
+unfold lift in |- *; auto with coc.
+Qed.
+
+  Hint Resolve red1_subst_l red1_subst_r: coc.
+
+
+  Lemma red_prod_prod :
+   forall u v t,
+   red (Prod u v) t ->
+   forall P : Prop,
+   (forall a b, t = Prod a b -> red u a -> red v b -> P) -> P.
+simple induction 1; intros.
+apply H0 with u v; auto with coc.
+
+apply H1; intros.
+inversion_clear H4 in H2.
+inversion H2.
+apply H3 with N1 b; auto with coc.
+apply trans_red with a; auto with coc.
+
+apply H3 with a N2; auto with coc.
+apply trans_red with b; auto with coc.
+Qed.
+
+
+  Lemma red_sort_sort : forall s t, red (Srt s) t -> t <> Srt s -> False.
+simple induction 1; intros; auto with coc.
+apply H1.
+generalize H2.
+case P; intros; try discriminate.
+inversion_clear H4.
+Qed.
+
+
+
+  Lemma one_step_conv_exp : forall M N, red1 M N -> conv N M.
+intros.
+apply trans_conv_exp with N; auto with coc.
+Qed.
+
+
+  Lemma red_conv : forall M N, red M N -> conv M N.
+simple induction 1; auto with coc.
+intros; apply trans_conv_red with P; auto with coc.
+Qed.
+
+  Hint Resolve one_step_conv_exp red_conv: coc.
+
+
+  Lemma sym_conv : forall M N, conv M N -> conv N M.
+simple induction 1; auto with coc.
+simple induction 2; intros; auto with coc.
+apply trans_conv_red with P0; auto with coc.
+
+apply trans_conv_exp with P0; auto with coc.
+
+simple induction 2; intros; auto with coc.
+apply trans_conv_red with P0; auto with coc.
+
+apply trans_conv_exp with P0; auto with coc.
+Qed.
+
+  Hint Immediate sym_conv: coc.
+
+
+  Lemma trans_conv_conv : forall M N P, conv M N -> conv N P -> conv M P.
+intros.
+generalize M H; elim H0; intros; auto with coc.
+apply trans_conv_red with P0; auto with coc.
+
+apply trans_conv_exp with P0; auto with coc.
+Qed.
+
+
+  Lemma conv_conv_prod :
+   forall a b c d, conv a b -> conv c d -> conv (Prod a c) (Prod b d).
+intros.
+apply trans_conv_conv with (Prod a d).
+elim H0; intros; auto with coc.
+apply trans_conv_red with (Prod a P); auto with coc.
+
+apply trans_conv_exp with (Prod a P); auto with coc.
+
+elim H; intros; auto with coc.
+apply trans_conv_red with (Prod P d); auto with coc.
+
+apply trans_conv_exp with (Prod P d); auto with coc.
+Qed.
+
+
+  Lemma conv_conv_lift :
+   forall a b n k, conv a b -> conv (lift_rec n a k) (lift_rec n b k).
+intros.
+elim H; intros; auto with coc.
+apply trans_conv_red with (lift_rec n P k); auto with coc.
+
+apply trans_conv_exp with (lift_rec n P k); auto with coc.
+Qed.
+ 
+
+  Lemma conv_conv_subst :
+   forall a b c d k,
+   conv a b -> conv c d -> conv (subst_rec a c k) (subst_rec b d k).
+intros.
+apply trans_conv_conv with (subst_rec a d k).
+elim H0; intros; auto with coc.
+apply trans_conv_red with (subst_rec a P k); auto with coc.
+
+apply trans_conv_exp with (subst_rec a P k); auto with coc.
+
+elim H; intros; auto with coc.
+apply trans_conv_conv with (subst_rec P d k); auto with coc.
+
+apply trans_conv_conv with (subst_rec P d k); auto with coc.
+apply sym_conv; auto with coc.
+Qed.
+
+  Hint Resolve conv_conv_prod conv_conv_lift conv_conv_subst: coc.
+
+
+  Lemma refl_par_red1 : forall M, par_red1 M M.
+simple induction M; auto with coc.
+Qed.
+
+  Hint Resolve refl_par_red1: coc.
+
+
+  Lemma red1_par_red1 : forall M N, red1 M N -> par_red1 M N.
+simple induction 1; auto with coc; intros.
+Qed.
+
+  Hint Resolve red1_par_red1: coc.
+
+
+  Lemma red_par_red : forall M N, red M N -> par_red M N.
+red in |- *; simple induction 1; intros; auto with coc.
+apply t_trans with P; auto with coc.
+Qed.
+
+
+  Lemma par_red_red : forall M N, par_red M N -> red M N.
+simple induction 1.
+simple induction 1; intros; auto with coc.
+apply trans_red with (App (Abs T M') N'); auto with coc.
+
+intros.
+apply trans_red_red with y; auto with coc.
+Qed.
+
+  Hint Resolve red_par_red par_red_red: coc.
+
+
+  Lemma par_red1_lift :
+   forall n a b,
+   par_red1 a b -> forall k, par_red1 (lift_rec n a k) (lift_rec n b k).
+simple induction 1; simpl in |- *; auto with coc.
+intros.
+rewrite distr_lift_subst; auto with coc.
+Qed.
+
+
+  Lemma par_red1_subst :
+   forall a b c d,
+   par_red1 a b ->
+   par_red1 c d -> forall k, par_red1 (subst_rec a c k) (subst_rec b d k).
+simple induction 2; simpl in |- *; auto with coc; intros.
+rewrite distr_subst; auto with coc.
+
+elim (lt_eq_lt_dec k n); auto with coc; intros.
+elim a0; intros; auto with coc.
+unfold lift in |- *.
+apply par_red1_lift; auto with coc.
+Qed.
+
+
+  Lemma inv_par_red_abs :
+   forall (P : Prop) T U x,
+   par_red1 (Abs T U) x ->
+   (forall T' U', x = Abs T' U' -> par_red1 U U' -> P) -> P.
+do 5 intro.
+inversion_clear H; intros.
+apply H with T' M'; auto with coc.
+Qed.
+
+  Hint Resolve par_red1_lift par_red1_subst: coc.
+
+
+
+  Lemma mem_sort_lift :
+   forall t n k s, mem_sort s (lift_rec n t k) -> mem_sort s t.
+simple induction t; simpl in |- *; intros; auto with coc.
+generalize H; elim (le_gt_dec k n); intros; auto with coc.
+inversion_clear H0.
+
+inversion_clear H1.
+apply mem_abs_l; apply H with n k; auto with coc.
+
+apply mem_abs_r; apply H0 with n (S k); auto with coc.
+
+inversion_clear H1.
+apply mem_app_l; apply H with n k; auto with coc.
+
+apply mem_app_r; apply H0 with n k; auto with coc.
+
+inversion_clear H1.
+apply mem_prod_l; apply H with n k; auto with coc.
+
+apply mem_prod_r; apply H0 with n (S k); auto with coc.
+Qed.
+
+
+  Lemma mem_sort_subst :
+   forall b a n s,
+   mem_sort s (subst_rec a b n) -> mem_sort s a \/ mem_sort s b.
+simple induction b; simpl in |- *; intros; auto with coc.
+generalize H; elim (lt_eq_lt_dec n0 n); intro.
+elim a0; intros.
+inversion_clear H0.
+
+left.
+apply mem_sort_lift with n0 0; auto with coc.
+
+intros.
+inversion_clear H0.
+
+inversion_clear H1.
+elim H with a n s; auto with coc.
+
+elim H0 with a (S n) s; auto with coc.
+
+inversion_clear H1.
+elim H with a n s; auto with coc.
+
+elim H0 with a n s; auto with coc.
+
+inversion_clear H1.
+elim H with a n s; auto with coc.
+
+elim H0 with a (S n) s; intros; auto with coc.
+Qed.
+
+
+  Lemma red_sort_mem : forall t s, red t (Srt s) -> mem_sort s t.
+intros.
+pattern t in |- *.
+apply red1_red_ind with (Srt s); auto with coc.
+do 4 intro.
+elim H0; intros.
+elim mem_sort_subst with M0 N 0 s; intros; auto with coc.
+
+inversion_clear H4; auto with coc.
+
+inversion_clear H4; auto with coc.
+
+inversion_clear H4; auto with coc.
+
+inversion_clear H4; auto with coc.
+
+inversion_clear H4; auto with coc.
+
+inversion_clear H4; auto with coc.
+Qed.
+
+
+
+  Lemma red_normal : forall u v, red u v -> normal u -> u = v.
+simple induction 1; auto with coc; intros.
+absurd (red1 u N); auto with coc.
+absurd (red1 P N); auto with coc.
+elim (H1 H3).
+unfold not in |- *; intro; apply (H3 N); auto with coc.
+Qed.
+
+
+
+  Lemma sn_red_sn : forall a b, sn a -> red a b -> sn b.
+unfold sn in |- *.
+simple induction 2; intros; auto with coc.
+apply Acc_inv with P; auto with coc.
+Qed.
+
+
+  Lemma commut_red1_subterm : commut _ subterm (transp _ red1).
+red in |- *.
+simple induction 1; intros.
+exists (Abs z B); auto with coc.
+
+exists (Abs A z); auto with coc.
+
+exists (App z B); auto with coc.
+
+exists (App A z); auto with coc.
+
+exists (Prod z B); auto with coc.
+
+exists (Prod A z); auto with coc.
+Qed.
+
+
+  Lemma subterm_sn : forall a, sn a -> forall b, subterm b a -> sn b.
+unfold sn in |- *.
+simple induction 1; intros.
+apply Acc_intro; intros.
+elim commut_red1_subterm with x b y; intros; auto with coc.
+apply H1 with x0; auto with coc.
+Qed.
+
+
+  Lemma sn_prod : forall A, sn A -> forall B, sn B -> sn (Prod A B).
+unfold sn in |- *.
+simple induction 1.
+simple induction 3; intros.
+apply Acc_intro; intros.
+inversion_clear H5; auto with coc.
+apply H1; auto with coc.
+apply Acc_intro; auto with coc.
+Qed.
+
+
+  Lemma sn_subst : forall T M, sn (subst T M) -> sn M.
+intros.
+cut (forall t, sn t -> forall m, t = subst T m -> sn m).
+intros.
+apply H0 with (subst T M); auto with coc.
+
+unfold sn in |- *.
+simple induction 1; intros.
+apply Acc_intro; intros.
+apply H2 with (subst T y); auto with coc.
+rewrite H3.
+unfold subst in |- *; auto with coc.
+Qed.
